AlgoleanTests.lean
@@ -9,4 +9,5 @@ public import AlgoleanTests.NaivePatternSearchExamples
 public import AlgoleanTests.ProgExamples
 public import AlgoleanTests.QueryExamples
 public import AlgoleanTests.RandomSampleExamples
+public import AlgoleanTests.WordRAMBinarySearchExamples
 public import AlgoleanTests.WordRAMExamples
